Core/Reduction/Congr.lean
@@ -5,88 +5,64 @@ import Core.Reduction.Definition
 open LeanSubst
 namespace Core
 -- Ctor2 Congr1
-@[simp]
-theorem Ctor2Variant.congr1_app : congr1 (app b) = true := by simp [congr1]
+-- @[simp]
+-- theorem Ctor2Variant.congr1_app : congr1 (app b) = true := by simp [congr1]
 
-@[simp]
-theorem Ctor2Variant.congr1_cast : congr1 cast = false := by simp [congr1]
+-- @[simp]
+-- theorem Ctor2Variant.congr1_cast : congr1 cast = false := by simp [congr1]
 
-@[simp]
-theorem Ctor2Variant.congr1_seq : congr1 seq = true := by simp [congr1]
+-- @[simp]
+-- theorem Ctor2Variant.congr1_apptc : congr1 apptc = true := by simp [congr1]
 
-@[simp]
-theorem Ctor2Variant.congr1_appc : congr1 appc = true := by simp [congr1]
+-- -- Ctor2 Congr2
+-- @[simp]
+-- theorem Ctor2Variant.congr2_app : congr2 (app .closed) = false := by simp [congr2]
 
-@[simp]
-theorem Ctor2Variant.congr1_apptc : congr1 apptc = true := by simp [congr1]
+-- @[simp]
+-- theorem Ctor2Variant.congr2_appo : congr2 (app .open) = true := by simp [congr2]
 
-@[simp]
-theorem Ctor2Variant.congr1_arrowc : congr1 arrowc = true := by simp [congr1]
+-- @[simp]
+-- theorem Ctor2Variant.congr2_cast : congr2 cast = true := by simp [congr2]
 
-@[simp]
-theorem Ctor2Variant.congr1_choice : congr1 choice = true := by simp [congr1]
+-- @[simp]
+-- theorem Ctor2Variant.congr2_apptc : congr2 apptc = true := by simp [congr2]
 
--- Ctor2 Congr2
-@[simp]
-theorem Ctor2Variant.congr2_app : congr2 (app .closed) = false := by simp [congr2]
+-- -- TyBind Congr
+-- @[simp]
+-- theorem TyBindVariant.congr_lamt : congr lamt = false := by simp [congr]
 
-@[simp]
-theorem Ctor2Variant.congr2_appo : congr2 (app .open) = true := by simp [congr2]
+-- @[simp]
+-- theorem TyBindVariant.congr_allc : congr allc = true := by simp [congr]
 
-@[simp]
-theorem Ctor2Variant.congr2_cast : congr2 cast = true := by simp [congr2]
+-- theorem Red.spine_congr_step :
+--   Red G t t' ->
+--   Red G (t.apply sp) (t'.apply sp)
+-- := by
+--   intro h
+--   induction sp generalizing t t'
+--   case nil => simp [Term.apply]; exact h
+--   case cons hd tl ih =>
+--     cases hd
+--     case type A =>
+--       simp [Term.apply]
+--       apply ih; apply Red.ctor1_congr h
+--     case term a =>
+--       simp [Term.apply]
+--       apply ih; apply Red.ctor2_congr1 _ h
+--       simp
+--     case oterm a =>
+--       simp [Term.apply]
+--       apply ih; apply Red.ctor2_congr1 _ h
+--       simp
 
-@[simp]
-theorem Ctor2Variant.congr2_seq : congr2 seq = true := by simp [congr2]
-
-@[simp]
-theorem Ctor2Variant.congr2_appc : congr2 appc = true := by simp [congr2]
-
-@[simp]
-theorem Ctor2Variant.congr2_apptc : congr2 apptc = true := by simp [congr2]
-
-@[simp]
-theorem Ctor2Variant.congr2_arrowc : congr2 arrowc = true := by simp [congr2]
-
-@[simp]
-theorem Ctor2Variant.congr2_choice : congr2 choice = true := by simp [congr2]
-
--- TyBind Congr
-@[simp]
-theorem TyBindVariant.congr_lamt : congr lamt = false := by simp [congr]
-
-@[simp]
-theorem TyBindVariant.congr_allc : congr allc = true := by simp [congr]
-
-theorem Red.spine_congr_step :
-  Red G t t' ->
-  Red G (t.apply sp) (t'.apply sp)
-:= by
-  intro h
-  induction sp generalizing t t'
-  case nil => simp [Term.apply]; exact h
-  case cons hd tl ih =>
-    cases hd
-    case type A =>
-      simp [Term.apply]
-      apply ih; apply Red.ctor1_congr h
-    case term a =>
-      simp [Term.apply]
-      apply ih; apply Red.ctor2_congr1 _ h
-      simp
-    case oterm a =>
-      simp [Term.apply]
-      apply ih; apply Red.ctor2_congr1 _ h
-      simp
-
-theorem Red.spine_congr :
-  Star (Red G) t t' ->
-  Star (Red G) (t.apply sp) (t'.apply sp)
-:= by
-  intro h
-  induction h
-  case _ => apply Star.refl
-  case _ y z h1 h2 ih =>
-    apply Star.step ih
-    apply spine_congr_step h2
+-- theorem Red.spine_congr :
+--   Star (Red G) t t' ->
+--   Star (Red G) (t.apply sp) (t'.apply sp)
+-- := by
+--   intro h
+--   induction h
+--   case _ => apply Star.refl
+--   case _ y z h1 h2 ih =>
+--     apply Star.step ih
+--     apply spine_congr_step h2
 end Core
